src/StarMalloc.fst
@@ -90,7 +90,9 @@ val memcpy_u8 (dest src: array U8.t) (n: US.t)
 
 module G = FStar.Ghost
 
-let realloc_vp (status: nat{status < 3})
+let return_status = x:nat{x < 3}
+
+let realloc_vp (status: return_status)
   (ptr: array U8.t)
   (new_ptr: array U8.t)
   (r: array U8.t)
@@ -107,11 +109,12 @@ let realloc_vp (status: nat{status < 3})
 
 #restart-solver
 
+
 #push-options "--z3rlimit 100 --compat_pre_typed_indexed_effects"
 let realloc (ptr: array U8.t) (new_size: US.t)
-  : Steel (array U8.t & (G.erased (x:nat{x < 3}) & G.erased (array U8.t)))
+  : Steel (array U8.t & G.erased (return_status & array U8.t))
   (null_or_varray ptr)
-  (fun r -> realloc_vp (G.reveal (fst (snd r))) ptr (snd (snd r)) (fst r))
+  (fun r -> realloc_vp (fst (G.reveal (snd r))) ptr (snd (G.reveal (snd r))) (fst r))
   (requires fun _ -> A.is_full_array ptr)
   (ensures fun _ r _ ->
     not (A.is_null (fst r)) ==> A.length (fst r) >= US.v new_size
@@ -126,7 +129,7 @@ let realloc (ptr: array U8.t) (new_size: US.t)
     change_equal_slprop
       (if A.is_null new_ptr then emp else A.varray new_ptr)
       (realloc_vp 0 (A.null #U8.t) (A.null #U8.t) new_ptr);
-    return (new_ptr, (G.hide 0, G.hide (A.null #U8.t)))
+    return (new_ptr, G.hide (0, A.null #U8.t))
   ) else (
     change_equal_slprop (null_or_varray ptr) (A.varray ptr);
     let new_ptr = malloc new_size in
@@ -141,7 +144,7 @@ let realloc (ptr: array U8.t) (new_size: US.t)
       change_equal_slprop
         (A.varray ptr)
         (realloc_vp 1 ptr (A.null #U8.t) (A.null #U8.t));
-      return (A.null #U8.t, (G.hide 1, G.hide (A.null #U8.t)))
+      return (A.null #U8.t, G.hide (1, A.null #U8.t))
     ) else (
       // The content of the memory block is preserved up to the
       // lesser of the new and old sizes, even if the block is
@@ -168,14 +171,14 @@ let realloc (ptr: array U8.t) (new_size: US.t)
         change_equal_slprop
           (null_or_varray new_ptr)
           (realloc_vp 0 ptr (A.null #U8.t) new_ptr);
-        return (new_ptr, (G.hide 0, G.hide (A.null #U8.t)))
+        return (new_ptr, G.hide (0, A.null #U8.t))
       ) else (
         change_equal_slprop
           (if b then emp else A.varray ptr) (null_or_varray ptr);
         change_equal_slprop
           (null_or_varray ptr `star` null_or_varray new_ptr)
           (realloc_vp 2 ptr new_ptr (A.null #U8.t));
-        return (A.null #U8.t, (G.hide 2, G.hide new_ptr))
+        return (A.null #U8.t, G.hide (2, new_ptr))
       )
     )
   )
